---
title: AMM12338
# author: dxdydz
date: 2023-06-23 10:15:00 -0400
categories: [AMM]
tags: [infinite series, integration, infinite products]
math: True
pin: False
---

## Problem - I. Mezo (China)

Prove

$$\int_0^\infty\frac{\cos(x)-1}{x(e^x-1)}\,\mathrm dx=\frac{1}{2}\ln\left(\frac{\pi}{\sinh(\pi)}\right).$$

## Solution

First we acquire two preliminary identities. In Euler's product for the sine

$$\frac{\sin(x)}{x}=\prod_{n=1}^\infty\left(1-\frac{x^2}{n^2\pi^2}\right)$$

we let $x=\pi i$ to get

$$\frac{\sinh(\pi)}{\pi}=\prod_{n=1}^\infty\left(1+\frac{1}{n^2}\right).$$

We are also interested in getting the value of

$$I(s)=\int_0^\infty\frac{\cos(x)-1}{x}e^{-sx}\,\mathrm dx,$$

which we find using the Feynman trick.

$$\begin{align*}    I'(s) &= \int_0^\infty(1-\cos(x))e^{-sx}\,\mathrm dx \\    &= \frac{1}{s}-\frac{s}{1+s^2}.\end{align*}$$

Then we have

$$\begin{align*}    I(s) &= \int_\infty^s I'(u) \,\mathrm du \\    &= \left[\ln(u)-\frac{1}{2}\ln(1+u^2)\right]\bigg\vert_\infty^s \\    &= \ln(s)-\frac{1}{2}\ln(1+s^2)-\lim_{u\to \infty}I(u) \\    &= -\frac{1}{2}\ln\left(1+\frac{1}{s^2}\right).\end{align*}$$

Finally,

$$\begin{align*}    \int_0^\infty\frac{\cos(x)-1}{x(e^x-1)}\,\mathrm dx &= \int_0^\infty\frac{(\cos(x)-1)e^{-x}}{x(1-e^{-x})}\,\mathrm dx \\    &= \sum_{n=1}^\infty\int_0^\infty\frac{\cos(x)-1}{x}e^{-nx}\,\mathrm dx,\;\;\text{monotone convergence} \\    &= -\frac{1}{2}\sum_{n=1}^\infty\ln\left(1+\frac{1}{n^2}\right) \\    &= \frac{1}{2}\ln\left(\prod_{n=1}^\infty\left(1+\frac{1}{n^2}\right)^{-1}\right) \\    &= \frac{1}{2}\ln\left(\frac{\pi}{\sinh(\pi)}\right).\end{align*}$$