---
title: AMM12256
# author: dxdydz
date: 2023-06-22 12:00:00 -0400
categories: [AMM]
tags: [infinite series, integration]
math: True
pin: False
---

## Problem - P. Bracken (USA)

Prove

$$\int_0^1\frac{\ln(1+x)\ln(1-x)}{x}\,\mathrm dx=-\frac{5\zeta(3)}{8}.$$

## Solution

Call the posed integral $I$ and define

$$J=\int_0^1\frac{1}{x}\ln^2\left(\frac{1-x}{1+x}\right)\,\mathrm dx.$$

Upon making the substitution $x=\frac{1-t}{1+t}$ we find that

$$\begin{align*}    J &= 2\int_0^1\frac{1+t}{1-t}\cdot\frac{1}{(1+t)^2}\ln^2(t)\,\mathrm dt \\      &= 2\int_0^1\frac{\ln^2(t)}{1-t^2}\,\mathrm dt \\      &= 2\int_0^1\ln^2(t)\sum_{n=0}^\infty t^{2n} dt, \\      &\qquad\text{by monotone convergence} \\      &= 2\sum_{n=0}^\infty\int_0^1\ln^2(t)t^{2n}\,\mathrm dt \\      &= 4\sum_{n=0}^\infty\frac{1}{(2n+1)^3} \\      &= \frac{7\zeta(3)}{2}.\end{align*}$$

In the above, the integral $\int_0^1\ln^2(t)t^\alpha\,\mathrm dt$ may be evaluated by differentiating $\int_0^1 t^\alpha\,\mathrm dt=\frac{1}{\alpha+1}$ under the integral sign twice. And the sum $\sum_{n=0}^\infty\frac{1}{(2n+1)^3}$ can be evaluated by considering $\sum_{n=1}^\infty\frac{1}{n^3}=\sum_{n=0}^\infty\frac{1}{(2n+1)^3}+\sum_{n=1}^\infty\frac{1}{(2n)^3}$.

Let

$$K=\int_0^1\frac{\ln^2(1-x^2)}{x}\,\mathrm dx.$$

If we make the change of variables $x=\sqrt{1-t}$ so that $\mathrm dx=\frac{-1}{2\sqrt{1-t}}\,\mathrm dt$ we get

$$\begin{align*}    K &= \frac{1}{2}\int_0^1\frac{\ln^2(t)}{1-t}\,\mathrm dt \\      &= \frac{1}{2}\int_0^1\ln^2(t)\sum_{n=0}^\infty t^n\,\mathrm dt, \\      &\qquad\text{by monotone convergence}\\      &= \sum_{n=0}^\infty\frac{1}{(n+1)^3} \\      &= \zeta(3).\end{align*}$$

Then

$$\begin{align*}    I &= \frac{1}{4}\int_0^1\frac{(\ln(1-x)+\ln(1+x))^2-(\ln(1-x)-\ln(1+x))^2}{x}\,\mathrm dx \\      &= \frac{1}{4}\left(\int_0^1\frac{(\ln(1-x)+\ln(1+x))^2}{x}\,\mathrm dx-\int_0^1\frac{(\ln(1-x)-\ln(1+x))^2}{x}\,\mathrm dx\right) \\      &= \frac{1}{4}(K-J) \\      &= -\frac{5\zeta(3)}{8}.\end{align*}$$