---
title: AMM12398
# author: dxdydz
date: 2023-11-04 19:40:00 -0400
categories: [American Mathematical Monthly Problems]
tags: [infinite series, infinite products]
math: True
pin: False
---

## Problem - L. Glasser (USA)

Evaluate

$$\sum_{n=0}^\infty\frac{1}{\sinh(2^n)}.$$

## Solution

First we show that

$$\prod_{n=1}^\infty\sqrt[2^n]{\tanh\left(2^{n-1}x\right)}=1-e^{-2x}.$$

Consider the auxilliary functions

$$f_{\pm}(t)=\prod_{n=0}^\infty(1\pm t^{2^n})^{1/2^n}.$$

Note that

$$\begin{align*}
f_+(t)f_-(t) &= \prod_{n=0}^\infty(1-t^{2^{n+1}})^{1/2^n} \\
&= \prod_{n=1}^\infty(1-t^{2^{n}})^{2/2^n} \\
&= \left(\frac{f_-(t)}{1-t}\right)^2
\end{align*}$$

so

$$\frac{f_-(t)}{f_+(t)}=(1-t)^2$$

and

$$\prod_{n=1}^\infty(1\pm t^{2^n})^{1/2^n}=\frac{f_\pm(t)}{1\pm t}.$$

It follows that

$$\frac{\prod_{n=1}^\infty(1- t^{2^n})^{1/2^n}}{\prod_{n=1}^\infty(1+ t^{2^n})^{1/2^n}}=1-t^2.$$

Letting $t=e^{x/2}$ yields the product

$$\prod_{n=1}^\infty\sqrt[2^n]{\tanh\left(2^{n-1}x\right)}=1-e^{-2x}.$$

that we were after. Taking the logarithmic derivative of each side of this product yields

$$\sum_{n=1}^\infty\frac{1}{\sinh(2^n x)}=\frac{2}{e^{2x}-1}$$

and upon setting $x=1$ we find that

$$\sum_{n=1}^\infty\frac{1}{\sinh(2^n)}=\frac{2}{e^{2}-1}.$$