---
title: AMM12273
# author: dxdydz
date: 2023-06-22 12:25:00 -0400
categories: [AMM]
tags: [infinite series, infinite products]
math: True
pin: False
---

## Problem - H. Ohtsuka (Japan)

For $s>1$, prove the following inequalities:

$$\sum_p\frac{1}{p^s-\frac{1}{2}}<\log(\zeta(s)),\,\sum_p\frac{1}{p^s}<\log\left(\frac{\zeta(s)}{\sqrt{\zeta(2s)}}\right),\,\sum_p\frac{1}{p^s+\frac{1}{2}}<\log\left(\frac{\zeta(s)}{\zeta(2s)}\right)$$

where all sums are taken over prime numbers $p$, and $\zeta(s)=\sum_{k=1}^\infty1/k^s$.

## Solution

We make use of the Euler product $\zeta(s)=\prod_p\frac{1}{1-1/p^s}$, $s>1$, and the Mercator series $\log(1+x)=\sum_{n=1}^\infty\frac{(-1)^{n+1}}{n}x^n$, $-1<x<1$, for all three inequalities.

\bigskip

### 1)

$$\begin{align*}    \log(\zeta(s)) &= -\sum_p\log\left(1-\frac{1}{p^s}\right)\\    &= \sum_p\sum_{n=1}^\infty\frac{1}{np^{ns}}\\    &>\sum_p\sum_{n=1}^\infty\frac{1}{2^{n-1}p^{ns}}\\    &=\sum_p\frac{2}{2p^s-1}\\    &=\sum_p\frac{1}{p^s-\frac{1}{2}}.\end{align*}$$

### 2)

$$\begin{align*}    \log\left(\frac{\zeta(s)}{\sqrt{\zeta(2s)}}\right) &= \sum_p\left(-\log\left(1-\frac{1}{p^s}\right)+\frac{1}{2}\log\left(1-\frac{1}{p^{2s}}\right)\right)\\    &= \sum_p\left(-\log\left(1-\frac{1}{p^s}\right)+\frac{1}{2}\log\left(\left(1-\frac{1}{p^{s}}\right)\left(1+\frac{1}{p^{s}}\right)\right)\right)\\    &=\frac{1}{2}\sum_p\left(\log\left(1+\frac{1}{p^s}\right)-\log\left(1-\frac{1}{p^s}\right)\right)\\    &=\frac{1}{2}\sum_p\left(\sum_{n=1}^\infty\frac{(-1)^{n+1}}{np^{ns}}+\sum_{n=1}^\infty\frac{1}{np^{ns}}\right)\\    &= \frac{1}{2}\sum_p\sum_{n=0}^\infty\frac{2}{(2n+1)p^{(2n+1)s}}\\    &>\sum_p\frac{1}{p^s}.\end{align*}$$

### 3)

$$\begin{align*}    \log\left(\frac{\zeta(s)}{\zeta(2s)}\right) &= \sum_p\left(-\log\left(1-\frac{1}{p^s}\right)+\log\left(1-\frac{1}{p^{2s}}\right)\right)\\    &= \sum_p\left(\log\left(\left(1-\frac{1}{p^{s}}\right)\left(1+\frac{1}{p^{s}}\right)\right)-\log\left(1-\frac{1}{p^s}\right)\right)\\    &= \sum_p\log\left(1+\frac{1}{p^{s}}\right)\\    &=\sum_p\sum_{n=1}^\infty\frac{(-1)^{n+1}}{np^{ns}}\\    &>\sum_p\sum_{n=1}^\infty\frac{(-1)^{n+1}}{2^{n-1}p^{ns}}\\    &=\sum_p\frac{2}{2p^s+1}\\    &=\sum_p\frac{1}{p^s+\frac{1}{2}}.\end{align*}$$